PurelyFunctionalDataStructures/Chapter03/Heap.v
@@ -1,0 +1,224 @@
+Class ordered (T : Type) :=
+  { eq  : T -> T -> bool
+  ; lt  : T -> T -> bool
+  ; leq : T -> T -> bool
+
+  ; eq_sym
+      : forall (t1 t2 : T)
+      , eq t1 t2 = eq t2 t1
+  ; lt_asym
+      : forall (t1 t2 : T) (b : bool)
+      , lt t1 t2 = true -> lt t2 t1 = false
+  ; eq_implies_leq
+      : forall (t1 t2 : T)
+      , eq t1 t2 = true -> leq t1 t2 = true
+  ; lt_implies_leq
+      : forall (t1 t2 : T)
+      , lt t1 t2 = true -> leq t1 t2 = true
+  ; lt_not_eq
+      : forall (t1 t2 : T)
+      , lt t1 t2 = true -> eq t1 t2 = false
+  }.
+
+Class heap (H : Type) (E : Type) `{o : ordered E} : Type :=
+  { empty     : H
+  ; isEmpty   : H -> bool
+  ; insert    : E -> H -> H
+  ; merge     : H -> H -> H
+  ; findMin   : H -> option E
+  ; deleteMin : H -> option H
+
+  ; empty_is_empty
+      : isEmpty empty = true
+  ; non_empty_is_not_empty
+      : forall (h : H) (e : E)
+      , isEmpty (insert e h) = true
+  ; merge_empty_left
+      : forall (h : H)
+      , merge empty h = h
+  ; merge_empty_right
+      : forall (h : H)
+      , merge h empty = h
+  ; empty_findMin
+      : findMin empty = None
+  ; empty_deleteMin
+      : deleteMin empty = None
+  ; insert_min
+      : forall (h : H) (e1 e2 : E)
+      , findMin h = Some e1 -> lt e2 e1 = true -> findMin (insert e2 h) = Some e2
+  ; insert_non_min
+      : forall (h : H) (e1 e2 : E)
+      , findMin h = Some e1 -> lt e2 e1 = false -> findMin (insert e2 h) = Some e1
+  ; merge_min_left
+      : forall (h1 h2 : H) (e1 e2 : E)
+      , findMin h1 = Some e1 -> findMin h2 = Some e2 -> lt e1 e2 = true -> findMin (merge h1 h2) = Some e1
+  ; merge_min_right
+      : forall (h1 h2 : H) (e1 e2 : E)
+      , findMin h1 = Some e1 -> findMin h2 = Some e2 -> lt e2 e1 = true -> findMin (merge h1 h2) = Some e2
+  ; delete_min
+      : forall (h1 h2 : H) (e1 e2 : E)
+      , findMin h1 = Some e1 -> lt e2 e1 = true -> deleteMin (insert e2 h1) = Some h2 -> findMin h2 = Some e1
+  }.
+
+Require Import Arith.
+
+Inductive leftish_heap (E : Type) : Type :=
+  | Empty : leftish_heap E
+  | Node  : nat -> E -> leftish_heap E -> leftish_heap E -> leftish_heap E
+  .
+
+Definition lh_empty {E : Type} : leftish_heap E :=
+  Empty E.
+
+Definition lh_isEmpty {E : Type} (h : leftish_heap E) : bool :=
+  match h with
+    | Empty _         => true
+    | Node  _ _ _ _ _ => false
+  end.
+
+Definition lh_findMin {E : Type} `{o : ordered E} (h : leftish_heap E) : option E :=
+  match h with
+    | Empty _ => None
+    | Node _ _ x _ _ => Some x
+  end.
+
+Definition rank {E : Type} (e : leftish_heap E) : nat :=
+  match e with
+    | Empty _         => 0
+    | Node  _ r _ _ _ => r
+  end.
+
+(* Cannot guess decreasing argument of fix. *)
+(* Definition makeT {E : Type} (x : E) (a : leftish_heap E) (b : leftish_heap E) : leftish_heap E :=
+  if (rank b) <? (rank a)
+    then Node E (rank b + 1) x a b
+    else Node E (rank a + 1) x b a.
+
+Fixpoint merge {E : Type} `{o : ordered E} (e1 : leftish_heap E) (e2 : leftish_heap E) : leftish_heap E :=
+  match e1, e2 with
+    | h, Empty _ => h
+    | Empty _, h => h
+    | Node _ _ x a1 b1 as h1, Node _ _ y a2 b2 as h2 =>
+        if leq x y
+          then makeT x a1 (merge b1 h2)
+          else makeT y a2 (merge h1 b2)
+  end. *)
+
+Fixpoint lh_merge {E : Type} `{o : ordered E} (e1 : leftish_heap E) (e2 : leftish_heap E) : leftish_heap E :=
+  match e1, e2 with
+    | h, Empty _ => h
+    | Empty _, h => h
+    | Node _ _ x a1 b1 as h1, Node _ _ y a2 b2 as h2 =>
+        if leq x y
+          then (let a := a1 in
+                let b := lh_merge b1 h2 in
+                let ra := rank a in
+                let rb := rank b
+                in if rank b <? rank a
+                    then Node E (rb + 1) x a b
+                    else Node E (ra + 1) x b a)
+          else (let a := a1 in
+                let b := lh_merge b1 h2 in
+                let ra := rank a in
+                let rb := rank b
+                in if rank b <? rank a
+                    then Node E (rb + 1) x a b
+                    else Node E (ra + 1) x b a)
+  end.
+
+Definition lh_insert {E : Type} `{o : ordered E} (x : E) (h : leftish_heap E) : leftish_heap E :=
+  lh_merge (Node E 1 x (Empty E) (Empty E)) h.
+
+Definition lh_deleteMin {E : Type} `{o : ordered E} (h : leftish_heap E) : option (leftish_heap E) :=
+  match h with
+    | Empty _         => None
+    | Node  _ _ x a b => Some (lh_merge a b)
+  end.
+
+Theorem lh_empty_is_empty
+  : forall (E : Type)
+  , @lh_isEmpty E lh_empty = true.
+Proof.
+Admitted.
+
+Theorem lh_non_empty_is_not_empty
+  : forall (E : Type) (o : ordered E) (h : leftish_heap E) (e : E)
+  , lh_isEmpty (lh_insert e h) = true.
+Proof.
+Admitted.
+
+Theorem lh_merge_empty_left
+  : forall (E : Type) (o : ordered E) (h : leftish_heap E)
+  , lh_merge lh_empty h = h.
+Proof.
+Admitted.
+
+Theorem lh_merge_empty_right
+  : forall (E : Type) (o : ordered E) (h : leftish_heap E)
+  , lh_merge h lh_empty = h.
+Proof.
+Admitted.
+
+Theorem lh_empty_findMin
+  : forall (E : Type) (o : ordered E)
+  , lh_findMin lh_empty = None.
+Proof.
+Admitted.
+
+Theorem lh_empty_deleteMin
+  : forall (E : Type) (o : ordered E)
+  , lh_deleteMin lh_empty = None.
+Proof.
+Admitted.
+
+Theorem lh_insert_min
+  : forall (E : Type) (o : ordered E) (h : leftish_heap E) (e1 e2 : E)
+  , lh_findMin h = Some e1 -> lt e2 e1 = true -> lh_findMin (lh_insert e2 h) = Some e2.
+Proof.
+Admitted.
+
+Theorem lh_insert_non_min
+  : forall (E : Type) (o : ordered E) (h : leftish_heap E) (e1 e2 : E)
+  , lh_findMin h = Some e1 -> lt e2 e1 = false -> lh_findMin (lh_insert e2 h) = Some e1.
+Proof.
+Admitted.
+
+Theorem lh_merge_min_left
+  : forall (E : Type) (o : ordered E) (h1 h2 : leftish_heap E) (e1 e2 : E)
+  , lh_findMin h1 = Some e1 -> lh_findMin h2 = Some e2 -> lt e1 e2 = true -> lh_findMin (lh_merge h1 h2) = Some e1.
+Proof.
+Admitted.
+
+Theorem lh_merge_min_right
+  : forall (E : Type) (o : ordered E) (h1 h2 : leftish_heap E) (e1 e2 : E)
+  , lh_findMin h1 = Some e1 -> lh_findMin h2 = Some e2 -> lt e2 e1 = true -> lh_findMin (lh_merge h1 h2) = Some e2.
+Proof.
+Admitted.
+
+Theorem lh_delete_min
+  : forall (E : Type) (o : ordered E) (h1 h2 : leftish_heap E) (e1 e2 : E)
+  , lh_findMin h1 = Some e1 -> lt e2 e1 = true -> lh_deleteMin (lh_insert e2 h1) = Some h2 -> lh_findMin h2 = Some e1.
+Proof.
+Admitted.
+
+(* TODO: Figure out how to instanciate this *)
+(* Instance leftish {E : Type} `{o : ordered E} : heap (leftish_heap E) E :=
+  { empty     := lh_empty
+  ; isEmpty   := lh_isEmpty
+  ; insert    := lh_insert
+  ; merge     := lh_merge
+  ; findMin   := lh_findMin
+  ; deleteMin := lh_deleteMin
+
+  ; empty_is_empty          := lh_empty_is_empty
+  ; non_empty_is_not_empty  := lh_non_empty_is_not_empty
+  ; merge_empty_left        := lh_merge_empty_left
+  ; merge_empty_right       := lh_merge_empty_right
+  ; empty_findMin           := lh_empty_findMin
+  ; empty_deleteMin         := lh_empty_deleteMin
+  ; insert_min              := lh_insert_min
+  ; insert_non_min          := lh_insert_non_min
+  ; merge_min_left          := lh_merge_min_left
+  ; merge_min_right         := lh_merge_min_right
+  ; delete_min              := lh_delete_min
+  }. *)
